specs/L1Nullifier/L1Nullifier/Common/for_6136861723173755809_user.lean
@@ -12,31 +12,39 @@ section
 
 open Clear EVMState Ast Expr Stmt FunctionDefinition State Interpreter ExecLemmas OutOfFuelLemmas Abstraction YulNotation PrimOps ReasoningPrinciple Utilities 
 
-def ACond_for_6136861723173755809 (s₀ : State) : Literal := sorry 
-def APost_for_6136861723173755809 (s₀ s₉ : State) : Prop := sorry
-def ABody_for_6136861723173755809 (s₀ s₉ : State) : Prop := sorry
-def AFor_for_6136861723173755809 (s₀ s₉ : State) : Prop := sorry
+def ACond_for_6136861723173755809 (s₀ : State) : Literal := fromBool (s₀["src"]!! < s₀["srcEnd"]!!)
+def APost_for_6136861723173755809 (s₀ s₉ : State) : Prop := True
+def ABody_for_6136861723173755809 (s₀ s₉ : State) : Prop := True
+def AFor_for_6136861723173755809 (s₀ s₉ : State) : Prop := True
 
 lemma for_6136861723173755809_cond_abs_of_code {s₀ fuel} : eval fuel for_6136861723173755809_cond (s₀) = (s₀, ACond_for_6136861723173755809 (s₀)) := by
   unfold eval ACond_for_6136861723173755809
-  sorry
+  simp [for_6136861723173755809_cond, evalArgs, head', reverse', Var', Lit', PrimCall', evalPrimCall]
+  rw [EVMLt']
+  simp [fromBool]
 
 lemma for_6136861723173755809_concrete_of_post_abs {s₀ s₉ : State} :
   Spec for_6136861723173755809_post_concrete_of_code s₀ s₉ →
   Spec APost_for_6136861723173755809 s₀ s₉ := by
-  sorry
+  unfold APost_for_6136861723173755809
+  rcases s₀ with ⟨evm, varstore⟩ | _ | _ <;> aesop_spec
 
 lemma for_6136861723173755809_concrete_of_body_abs {s₀ s₉ : State} :
   Spec for_6136861723173755809_body_concrete_of_code s₀ s₉ →
   Spec ABody_for_6136861723173755809 s₀ s₉ := by
-  sorry
+  unfold ABody_for_6136861723173755809
+  rcases s₀ with ⟨evm, varstore⟩ | _ | _ <;> aesop_spec
 
-lemma AZero_for_6136861723173755809 : ∀ s₀, isOk s₀ → ACond_for_6136861723173755809 (👌 s₀) = 0 → AFor_for_6136861723173755809 s₀ s₀ := sorry
+lemma AZero_for_6136861723173755809 : ∀ s₀, isOk s₀ → ACond_for_6136861723173755809 (👌 s₀) = 0 → AFor_for_6136861723173755809 s₀ s₀ := by
+  intro s₀ _ _; trivial
 lemma AOk_for_6136861723173755809 : ∀ s₀ s₂ s₄ s₅, isOk s₀ → isOk s₂ → ¬ ❓ s₅ → ¬ ACond_for_6136861723173755809 s₀ = 0 → ABody_for_6136861723173755809 s₀ s₂ → APost_for_6136861723173755809 s₂ s₄ → Spec AFor_for_6136861723173755809 s₄ s₅ → AFor_for_6136861723173755809 s₀ s₅
-:= sorry
-lemma AContinue_for_6136861723173755809 : ∀ s₀ s₂ s₄ s₅, isOk s₀ → isContinue s₂ → ¬ ACond_for_6136861723173755809 s₀ = 0 → ABody_for_6136861723173755809 s₀ s₂ → Spec APost_for_6136861723173755809 (🧟s₂) s₄ → Spec AFor_for_6136861723173755809 s₄ s₅ → AFor_for_6136861723173755809 s₀ s₅ := sorry
-lemma ABreak_for_6136861723173755809 : ∀ s₀ s₂, isOk s₀ → isBreak s₂ → ¬ ACond_for_6136861723173755809 s₀ = 0 → ABody_for_6136861723173755809 s₀ s₂ → AFor_for_6136861723173755809 s₀ (🧟s₂) := sorry
-lemma ALeave_for_6136861723173755809 : ∀ s₀ s₂, isOk s₀ → isLeave s₂ → ¬ ACond_for_6136861723173755809 s₀ = 0 → ABody_for_6136861723173755809 s₀ s₂ → AFor_for_6136861723173755809 s₀ s₂ := sorry
+:= by intro s₀ s₂ s₄ s₅ _ _ _ _ _ _ _; trivial
+lemma AContinue_for_6136861723173755809 : ∀ s₀ s₂ s₄ s₅, isOk s₀ → isContinue s₂ → ¬ ACond_for_6136861723173755809 s₀ = 0 → ABody_for_6136861723173755809 s₀ s₂ → Spec APost_for_6136861723173755809 (🧟s₂) s₄ → Spec AFor_for_6136861723173755809 s₄ s₅ → AFor_for_6136861723173755809 s₀ s₅ := by
+  intro s₀ s₂ s₄ s₅ _ _ _ _ _ _; trivial
+lemma ABreak_for_6136861723173755809 : ∀ s₀ s₂, isOk s₀ → isBreak s₂ → ¬ ACond_for_6136861723173755809 s₀ = 0 → ABody_for_6136861723173755809 s₀ s₂ → AFor_for_6136861723173755809 s₀ (🧟s₂) := by
+  intro s₀ s₂ _ _ _ _; trivial
+lemma ALeave_for_6136861723173755809 : ∀ s₀ s₂, isOk s₀ → isLeave s₂ → ¬ ACond_for_6136861723173755809 s₀ = 0 → ABody_for_6136861723173755809 s₀ s₂ → AFor_for_6136861723173755809 s₀ s₂ := by
+  intro s₀ s₂ _ _ _ _; trivial
 
 end
 
