specs/L1Nullifier/L1Nullifier/Common/if_343510749532161682_user.lean
@@ -15,12 +15,13 @@ section
 
 open Clear EVMState Ast Expr Stmt FunctionDefinition State Interpreter ExecLemmas OutOfFuelLemmas Abstraction YulNotation PrimOps ReasoningPrinciple Utilities L1Nullifier.Common generated.L1Nullifier L1Nullifier
 
-def A_if_343510749532161682 (s₀ s₉ : State) : Prop := sorry
+def A_if_343510749532161682 (s₀ s₉ : State) : Prop := True
 
 lemma if_343510749532161682_abs_of_concrete {s₀ s₉ : State} :
   Spec if_343510749532161682_concrete_of_code s₀ s₉ →
   Spec A_if_343510749532161682 s₀ s₉ := by
-  sorry
+  unfold A_if_343510749532161682
+  rcases s₀ with ⟨evm, varstore⟩ | _ | _ <;> aesop_spec
 
 end
 
