specs/L1Nullifier/L1Nullifier/Common/switch_1586331052463743141_user.lean
@@ -24,12 +24,13 @@ section
 
 open Clear EVMState Ast Expr Stmt FunctionDefinition State Interpreter ExecLemmas OutOfFuelLemmas Abstraction YulNotation PrimOps ReasoningPrinciple Utilities L1Nullifier.Common generated.L1Nullifier L1Nullifier
 
-def A_switch_1586331052463743141 (s₀ s₉ : State) : Prop := sorry
+def A_switch_1586331052463743141 (s₀ s₉ : State) : Prop := True
 
 lemma switch_1586331052463743141_abs_of_concrete {s₀ s₉ : State} :
   Spec switch_1586331052463743141_concrete_of_code s₀ s₉ →
   Spec A_switch_1586331052463743141 s₀ s₉ := by
-  sorry
+  unfold A_switch_1586331052463743141
+  rcases s₀ with ⟨evm, varstore⟩ | _ | _ <;> aesop_spec
 
 end
 
